src/lowparse/LowParse.Spec.Endianness.fst
@@ -51,20 +51,6 @@ let big_endian_lex_compare_eq
     E.n_to_be_inj n x y
   end else ()
 
-let rec seq_to_list_append
-  (#t: Type)
-  (s1 s2: Seq.seq t)
-: Lemma
-  (ensures (Seq.seq_to_list (s1 `Seq.append` s2) == Seq.seq_to_list s1 `List.Tot.append` Seq.seq_to_list s2))
-  (decreases (Seq.length s1))
-= if Seq.length s1 = 0
-  then begin
-    assert ((s1 `Seq.append` s2) `Seq.equal` s2)
-  end else begin
-    assert (Seq.slice (s1 `Seq.append` s2) 1 (Seq.length (s1 `Seq.append` s2)) `Seq.equal` (Seq.slice s1 1 (Seq.length s1) `Seq.append` s2));
-    seq_to_list_append (Seq.slice s1 1 (Seq.length s1)) s2
-  end
-
 let rec big_endian_lex_compare_aux
   (n: nat)
   (compare: (U8.t -> U8.t -> int))
